Refactor code for even/odd

theories/Infra/FreshGenInst.v
@@ -1,4 +1,4 @@
-Require Import Util CSet MapInjectivity NaturalRep FreshGen FreshNR.
+Require Import Util CSet MapInjectivity NaturalRep FreshGen FreshNR Even.
 
 Set Implicit Arguments.
 
@@ -59,51 +59,6 @@ Lemma FGS_fast_pos : FreshGenSpec FG_fast_pos.
       eauto with typeclass_instances.
 Qed.
 
-Definition next_even (n:nat) := if [even n] then n else S n.
-
-Lemma next_even_even n
-  : even (next_even n).
-Proof.
-  unfold next_even; cases; eauto.
-  edestruct (even_or_successor n); eauto.
-Qed.
-
-Lemma even_add x y
-  : even x
-    -> even y
-    -> even (x + y).
-Proof.
-  revert y. pattern x.
-  eapply size_induction with (f:=id); intros.
-  destruct x0; simpl; eauto.
-  destruct x0; simpl; eauto.
-  eapply H; eauto. unfold id. omega.
-Qed.
-
-Lemma even_max x y
-  : even x
-    -> even y
-    -> even (max x y).
-Proof.
-  intros.
-  decide (x < y).
-  - rewrite max_r; try omega; eauto.
-  - rewrite max_l; try omega; eauto.
-Qed.
-
-Lemma even_mult2 x
-  : even (2 * x).
-Proof.
-  pattern x.
-  eapply size_induction with (f:=id); intros.
-  destruct x0; simpl; eauto.
-  destruct x0; simpl; eauto. rewrite plus_comm. simpl.
-  rewrite <- plus_assoc. simpl.
-  exploit (H x0).
-  - unfold id. omega.
-  - simpl in H0. setoid_rewrite plus_comm in H0 at 2. simpl in *. eauto.
-Qed.
-
 Lemma NoDup_inj A `{OrderedType A} B `{OrderedType B} (L:list A) (f:A -> B)
       `{Proper _ (_eq ==> _eq) f}
   : NoDupA _eq L
@@ -145,47 +100,6 @@ Proof.
   intro.
   rewrite InA_in in H2.
   eapply in_range_x in H2. nr. omega.
-Qed.
-
-
-Definition even_pos_fast (p:positive) :=
-  match p with
-  | (p'~1)%positive => true
-  | (p'~0)%positive => false
-  | _ => true
-  end.
-
-Lemma even_pos_fast_succ p
-  : even_pos_fast (Pos.succ p) = negb (even_pos_fast p).
-Proof.
-  unfold even_pos_fast.
-  destruct p; simpl.
-  - reflexivity.
-  - reflexivity.
-  - reflexivity.
-Qed.
-
-Lemma even_pos_fast_correct p
-  : even (asNat p) = even_pos_fast p.
-Proof.
-  induction p using Pos.peano_ind.
-  - simpl. eauto.
-  - rewrite even_pos_fast_succ.
-    change Pos.succ with (@succ positive _ _ _).
-    nr. rewrite <- IHp.
-    rewrite even_not_even. simpl. reflexivity.
-Qed.
-
-Definition next_even_pos (n:positive) :=
-  if [even_pos_fast n] then n else succ n.
-
-Lemma next_even_pos_even n
-  : even (asNat (next_even_pos n)).
-Proof.
-  unfold next_even_pos.
-  rewrite <- even_pos_fast_correct.
-  cases; eauto. nr.
-  edestruct (even_or_successor (asNat n)); eauto.
 Qed.
 
 
