theories/Infra/Even.v
@@ -1,0 +1,118 @@
+Require Import Util NaturalRep.
+
+
+Fixpoint even (n:nat) : bool :=
+  match n with
+  | 0 => true
+  | S 0 => false
+  | S (S n) => even n
+  end.
+
+Lemma even_or_successor x
+  : even x \/ even (1 + x).
+Proof.
+  induction x; eauto.
+  destruct IHx; eauto.
+Qed.
+
+Definition odd := (fun x => negb (even x)).
+
+Lemma even_or_odd (x:nat)
+  : even x + odd x.
+Proof.
+  unfold odd. destruct (even x); eauto.
+Qed.
+
+Lemma even_not_even x
+  : even x = negb (even (S x)).
+Proof.
+  general induction x; eauto.
+  - simpl even at 2.
+    destruct (even x); destruct (even (S x)); simpl in *; intuition.
+Qed.
+
+Definition next_even (n:nat) := if [even n] then n else S n.
+
+Lemma next_even_even n
+  : even (next_even n).
+Proof.
+  unfold next_even; cases; eauto.
+  edestruct (even_or_successor n); eauto.
+Qed.
+
+Lemma even_add x y
+  : even x
+    -> even y
+    -> even (x + y).
+Proof.
+  revert y. pattern x.
+  eapply size_induction with (f:=id); intros.
+  destruct x0; simpl; eauto.
+  destruct x0; simpl; eauto.
+  eapply H; eauto. unfold id. omega.
+Qed.
+
+Lemma even_max x y
+  : even x
+    -> even y
+    -> even (max x y).
+Proof.
+  intros.
+  decide (x < y).
+  - rewrite max_r; try omega; eauto.
+  - rewrite max_l; try omega; eauto.
+Qed.
+
+Lemma even_mult2 x
+  : even (2 * x).
+Proof.
+  pattern x.
+  eapply size_induction with (f:=id); intros.
+  destruct x0; simpl; eauto.
+  destruct x0; simpl; eauto. rewrite plus_comm. simpl.
+  rewrite <- plus_assoc. simpl.
+  exploit (H x0).
+  - unfold id. omega.
+  - simpl in H0. setoid_rewrite plus_comm in H0 at 2. simpl in *. eauto.
+Qed.
+
+
+Definition even_pos_fast (p:positive) :=
+  match p with
+  | (p'~1)%positive => true
+  | (p'~0)%positive => false
+  | _ => true
+  end.
+
+Lemma even_pos_fast_succ p
+  : even_pos_fast (Pos.succ p) = negb (even_pos_fast p).
+Proof.
+  unfold even_pos_fast.
+  destruct p; simpl.
+  - reflexivity.
+  - reflexivity.
+  - reflexivity.
+Qed.
+
+Lemma even_pos_fast_correct p
+  : even (asNat p) = even_pos_fast p.
+Proof.
+  induction p using Pos.peano_ind.
+  - simpl. eauto.
+  - rewrite even_pos_fast_succ.
+    change Pos.succ with (@succ positive _ _ _).
+    nr. rewrite <- IHp.
+    rewrite even_not_even. simpl. reflexivity.
+Qed.
+
+Definition next_even_pos (n:positive) :=
+  if [even_pos_fast n] then n else succ n.
+
+Lemma next_even_pos_even n
+  : even (asNat (next_even_pos n)).
+Proof.
+  unfold next_even_pos.
+  rewrite <- even_pos_fast_correct.
+  cases; eauto. nr.
+  edestruct (even_or_successor (asNat n)); eauto.
+Qed.
